coq/CheriMemory/Memory_model.v
@@ -17,10 +17,10 @@ Set Implicit Arguments.
 Set Strict Implicit.
 Generalizable All Variables.
 
-Module Type Memory (A:PTRADDR) (B:PTRADDR_INTERVAL A).
+Module Type Memory (A:PTRADDR) (B:PTRADDR_INTERVAL A) (MC:Mem_common(A)(B)).
 
   Import A.
-  Include Mem_common(A)(B).
+  Import MC.
 
   (* Module interface below *)
 
